Translation/Term/Lemmas.lean
@@ -12,19 +12,22 @@ import Translation.Ty.Lemmas
 import Translation.Ty
 import Translation.Term
 import Translation.Global
+import Core.Typing
+import Surface.Typing
+
+
+def Surface.TyEnv.translate (G : Core.GlobalEnv) (Δ : Core.KindEnv) (Γ : Surface.TyEnv) : Option (Core.TyEnv) := Γ.mapM (·.translate G Δ )
 
 theorem Translation.Term.Sound (G : Surface.GlobalEnv) :
   ⊢s G ->
   G&Δ,Γ ⊢s t : T ->
-  Surface.Global.translateEnv G = some G' ->
-  Surface.Kind.translateEnv Δ = Δ' ->
-  Surface.Ty.translateEnv G' Δ' Γ = some Γ' ->
+  G.translate = some G' ->
+  Δ.translate = Δ' ->
+  Γ.translate G' Δ' = some Γ' ->
 
   (T.translate G' Δ' = some T' ∧
   t.translate G' Δ' Γ' = some t' ∧
   t'.Determined ∧
   G'&Δ',Γ' ⊢ t' : T') := by
-
-
 
 sorry
