Core/Reduction/Definition.lean
@@ -189,13 +189,13 @@ inductive Red (G : List Global) : Term -> Term -> Prop where
 
 notation:160 G:160 " ⊢ " t:160 " ~> " t':160 => Red G t t'
 
-inductive RedStar (G : Globals) : Term -> Term -> Prop where
+inductive RedStar (G : GlobalEnv) : Term -> Term -> Prop where
 | refl : RedStar G x x
 | step : RedStar G x y -> Red G y z -> RedStar G x z
 
 notation:160 G:160 " ⊢ " t:160 " ~>* " t':160 => RedStar G t t'
 
-inductive RedPlus (G : Globals) : Term -> Term -> Prop where
+inductive RedPlus (G : GlobalEnv) : Term -> Term -> Prop where
 | one : Red G x y -> RedPlus G x y
 | step : RedPlus G x y -> Red G y z -> RedPlus G x z
 
